doc: suggested revision to wf-rec preprocessing
Also fixes rendering issue with signature and proof states

Manual/RecursiveDefs/WF/PreprocessExample.lean
@@ -16,11 +16,19 @@ want to update it over and over again as we edit the large file.
 open Verso.Genre Manual
 open Lean.Elab.Tactic.GuardMsgs.WhitespaceMode
 
+set_option linter.constructorNameAsVariable false
+
 #doc (Manual) "Well-founded recursion preprocessing example (for inclusion elsewhere)" =>
 
-:::example "Preprocessing for a custom data type"
+::::example "Preprocessing for a custom data type"
 
-In this example, we define a new container-like data type (for homogeneous pairs), with a membership predicate, a map function and the necessary setup to allow well-founded recursion through that map function.
+This example demonstrates what is necessary to enable automatic well-founded recursion for a custom container type.
+The structure type {name}`Pair` is a homogeneous pair: it contains precisely two elements, both of which have the same type.
+It can be thought of as being similar to a list or array that always contains precisely two elements.
+
+As a container, {name}`Pair` can support a {name Pair.map}`map` operation.
+To support well-founded recursion in which recursive calls occur in the body of a function being mapped over a {name}`Pair`, some additional definitions are required, including a membership predicate, a theorem that relates the size of a member to the size of the containing pair, helpers to introduce and eliminate assumptions about membership, {attr}`wf_preprocess` rules to insert these helpers, and an extension to the {tactic}`decreasing_trivial` tactic.
+Each of these steps makes it easier to work with {name}`Pair`, but none are strictly necessary; there's no need to immediately implement all steps for every type.
 
 ```lean
 /-- A homogeneous pair -/
@@ -34,7 +42,7 @@ def Pair.map (f : α → β) (p : Pair α) : Pair β where
   snd := f p.snd
 ```
 
-To demonstrate the problem, we define a nested inductive data type for binary trees, and try to define a map function for it.
+Defining a nested inductive data type of binary trees that uses {name}`Pair` and attempting to define its {name Tree.map}`map` function demonstrates the need for preprocessing rules.
 
 ```lean
 /-- A binary tree defined using `Pair` -/
@@ -43,7 +51,7 @@ inductive Tree (α : Type u) where
   | node : Pair (Tree α) → Tree α
 ```
 
-Our definition of the map function fails:
+A straightforward definition of the {name Tree.map}`map` function fails:
 
 ```lean (error := true) (keep := false) (name := badwf)
 def Tree.map (f : α → β) : Tree α → Tree β
@@ -63,33 +71,41 @@ t' : Tree α
 ⊢ sizeOf t' < 1 + sizeOf p
 ```
 
+:::paragraph
 ```lean (show := false)
 section
 variable (t' : Tree α) (p : Pair (Tree α))
 ```
-Clearly the proof obligation is not solvable, as nothing connects `t'` to `p`. {TODO}[Cannot use `lean` here? Because this is in an example?]
+Clearly the proof obligation is not solvable, because nothing connects {lean}`t'` to {lean}`p`.
 ```lean (show := false)
 end
 ```
+:::
 
-The idiom to allow this function definition is to have a function that enriches the elements of the pair with the assertion that the elements are in the pair.
-For that we need a membership predicate.
+The standard idiom to enable this kind of function definition is to have a function that enriches each element of a collection with a proof that they are, in fact, elements of the collection.
+Stating this property requires a membership predicate.
 
 ```lean
 inductive Pair.Mem (p : Pair α) : α → Prop where
-| fst : Mem p p.fst
-| snd : Mem p p.snd
+  | fst : Mem p p.fst
+  | snd : Mem p p.snd
 
 instance : Membership α (Pair α) where
   mem := Pair.Mem
+```
 
-theorem Pair.size_lt_of_mem {α} [SizeOf α]
+Every inductive type automatically has a {name}`SizeOf` instance.
+An element of a collection should be smaller than the collection, but this fact must be proved before it can be used to construct a termination proof:
+
+```lean
+theorem Pair.sizeOf_lt_of_mem {α} [SizeOf α]
     {p : Pair α} {x : α} (h : x ∈ p) :
     sizeOf x < sizeOf p := by
   cases h <;> cases p <;> (simp; omega)
 ```
 
-Furthermore we introduce `attach` and `unattach` functions that enrich the elements of the pair with the assertion that they are in the pair, respectively remove that assertion.
+The next step is to define {name Pair.attach}`attach` and {name Pair.unattach}`unattach` functions that enrich the elements of the pair with a proof that they are elements of the pair, or remove said proof.
+Here, the type of {name}`Pair.unattach` is more general and can be used with any {ref "Subtype"}[subtype]; this is a typical pattern.
 
 ```lean
 def Pair.attach (p : Pair α) : Pair {x : α // x ∈ p} where
@@ -101,18 +117,24 @@ def Pair.unattach {P : α → Prop} :
   Pair.map Subtype.val
 ```
 
-This already allows us to define the `map` function by using `Pair.attach` explicitly:
+{name Tree.map}`Tree.map` can now be defined by using {name}`Pair.attach` and {name}`Pair.sizeOf_lt_of_mem` explicitly:
 
 ```lean (keep := false)
 def Tree.map (f : α → β) : Tree α → Tree β
   | leaf x => leaf (f x)
   | node p => node (p.attach.map (fun ⟨t', _⟩ => t'.map f))
 termination_by t => t
-decreasing_by have := Pair.size_lt_of_mem ‹_›; simp_all; omega
+decreasing_by
+  have := Pair.sizeOf_lt_of_mem ‹_›
+  simp_all +arith
+  omega
 ```
 
-We can use the preprocessing feature of well-founded recursion to automate the introduction of the {lean}`Pair.attach` function:
-
+This transformation can be made fully automatic.
+The preprocessing feature of well-founded recursion can be used to automate the introduction of the {lean}`Pair.attach` function.
+This is done in two stages.
+First, when {name}`Pair.map` is applied to one of the function's parameters, it is rewritten to an {name Pair.attach}`attach`/{name Pair.unattach}`unattach` composition.
+Then, when a function is mapped over the result of {name}`Pair.unattach`, the function is rewritten to accept the proof of membership and bring it into scope.
 ```lean
 @[wf_preprocess]
 theorem Pair.map_wfParam (f : α → β) (p : Pair α) :
@@ -123,19 +145,41 @@ theorem Pair.map_wfParam (f : α → β) (p : Pair α) :
 @[wf_preprocess]
 theorem Pair.map_unattach {P : α → Prop}
     (p : Pair (Subtype P)) (f : α → β) :
-    p.unattach.map f = p.map fun ⟨x, h⟩ => f (wfParam x) := by
+    p.unattach.map f =
+    p.map fun ⟨x, h⟩ =>
+      binderNameHint x f <|
+      f (wfParam x) := by
   cases p; simp [wfParam, Pair.unattach, Pair.map]
 ```
 
 Now the function body can be written without extra considerations, and the membership assumption is still available to the termination proof.
 
-```lean
+```lean (keep := false)
 def Tree.map (f : α → β) : Tree α → Tree β
   | leaf x => leaf (f x)
   | node p => node (p.map (fun t' => t'.map f))
 termination_by t => t
-decreasing_by have := Pair.size_lt_of_mem ‹_›; simp_all; omega
+decreasing_by
+  have := Pair.sizeOf_lt_of_mem ‹_›
+  simp_all
+  omega
 ```
 
+The proof can be made fully automatic by adding {name Pair.sizeOf_lt_of_mem}`sizeOf_lt_of_mem` to the {tactic}`decreasing_trivial` tactic, as is done for similar built-in theorems.
 
-:::
+```lean
+macro "sizeOf_pair_dec" : tactic =>
+  `(tactic| with_reducible
+    have := Pair.sizeOf_lt_of_mem ‹_›
+    omega
+    done)
+
+macro_rules | `(tactic| decreasing_trivial) => `(tactic| sizeOf_pair_dec)
+
+def Tree.map (f : α → β) : Tree α → Tree β
+  | leaf x => leaf (f x)
+  | node p => node (p.map (fun t' => t'.map f))
+termination_by t => t
+```
+
+::::
